autoclrs/ch15-dynamic-programming/c/CLRS.Ch15.LCS.C.BridgeLemmas.fst
@@ -21,3 +21,38 @@ let to_int_seq_index (s: seq (option I32.t)) (i: nat)
           (ensures Seq.index (to_int_seq s) i == I32.v (Some?.v (Seq.index s i)))
           [SMTPat (Seq.index (to_int_seq s) i)]
   = ()
+
+let to_int_seq_upd_some (s: seq (option I32.t)) (j: nat) (v: I32.t)
+  : Lemma (requires j < Seq.length s)
+          (ensures to_int_seq (Seq.upd s j (Some v)) == Seq.upd (to_int_seq s) j (I32.v v))
+          [SMTPat (to_int_seq (Seq.upd s j (Some v)))]
+  = assert (Seq.equal (to_int_seq (Seq.upd s j (Some v))) (Seq.upd (to_int_seq s) j (I32.v v)))
+
+open FStar.Mul
+
+(* Unconditional bridge for lcs_table_correct diagonal bound.
+   When i >= 1 /\ j >= 1, the diag value is at most i-1 (hence <= 999).
+   Called BEFORE the if block to avoid ghost-inside-branch issues. *)
+let lcs_table_diag_bound_opt (x y: seq int) (tbl: seq int) (m n i j: nat)
+  : Lemma
+      (requires
+        lcs_table_correct x y tbl m n i j /\
+        m == Seq.length x /\ n == Seq.length y /\
+        i <= m /\ j <= n /\
+        Seq.length tbl == (m + 1) * (n + 1))
+      (ensures
+        i >= 1 /\ j >= 1 ==>
+          Seq.index tbl ((i - 1) * (n + 1) + (j - 1)) <= i - 1)
+  = if i >= 1 && j >= 1 then
+      lcs_length_upper_bound x y (i - 1) (j - 1)
+    else ()
+
+(* Bridge: final table result equals lcs_length *)
+let lcs_table_result (x y: seq int) (tbl: seq int) (m n: nat)
+  : Lemma
+      (requires
+        lcs_table_correct x y tbl m n (m + 1) 0 /\
+        m == Seq.length x /\ n == Seq.length y)
+      (ensures
+        Seq.index tbl (m * (n + 1) + n) == lcs_length x y m n)
+  = ()
