autoclrs/ch15-dynamic-programming/c/RodCutting.fst
@@ -1,0 +1,175 @@
+module RodCutting
+open Pulse
+open Pulse.Lib.C
+#lang-pulse
+
+
+#restart-solver
+
+open Pulse.Lib.C.Array
+
+#restart-solver
+
+open CLRS.Ch15.RodCutting.Spec
+
+#restart-solver
+
+open CLRS.Ch15.RodCutting.C.BridgeLemmas
+
+#restart-solver
+
+fn func_rod_cutting (var_prices: (array Int32.t)) (var_n: SizeT.t) (var_r: (array Int32.t))
+  requires
+    exists* (val_prices_0: (Seq.seq (option Int32.t))) (val_prices_1: (nat->prop)).
+    ((array_pts_to var_prices 1.0R val_prices_0 val_prices_1))
+  requires
+    exists* (val_r_0: (Seq.seq (option Int32.t))) (val_r_1: (nat->prop)).
+    ((array_pts_to var_r 1.0R val_r_0 val_r_1))
+  requires (with_pure ((reveal (length_of var_prices)) = (SizeT.v var_n)))
+  requires (with_pure ((reveal (length_of var_r)) = ((SizeT.v var_n) + 1)))
+  requires (with_pure ((SizeT.v var_n) <= 1000))
+  requires
+    (with_pure
+      (forall
+        (var_i: SizeT.t).
+        ((var_n `SizeT.lte` var_i) ||
+          ((0 <= (id #int (Int32.v ((array_read var_prices var_i))))) &&
+            ((id #int (Int32.v ((array_read var_prices var_i)))) <= 1000000)))))
+  returns return_1 : unit
+  ensures
+    exists* (val_prices_0: (Seq.seq (option Int32.t))) (val_prices_1: (nat->prop)).
+    ((array_pts_to var_prices 1.0R val_prices_0 val_prices_1))
+  ensures
+    exists* (val_r_0: (Seq.seq (option Int32.t))) (val_r_1: (nat->prop)).
+    ((array_pts_to var_r 1.0R val_r_0 val_r_1))
+  ensures (with_pure ((reveal (length_of var_prices)) = (SizeT.v var_n)))
+  ensures (with_pure ((reveal (length_of var_r)) = ((SizeT.v var_n) + 1)))
+  ensures (with_pure (Int32.v (array_read var_r 0sz) = 0))
+  ensures
+    (with_pure
+      (forall
+        (var_k: SizeT.t).
+        ((var_n `SizeT.lt` var_k) || (0 <= (id #int (Int32.v ((array_read var_r var_k))))))))
+  ensures
+    (with_pure
+      (forall
+        (var_k: SizeT.t).
+        ((var_n `SizeT.lt` var_k) ||
+          (Int32.v (array_read var_r var_k) <= 1000000 * SizeT.v var_k))))
+  ensures
+    (with_pure (
+id #int (Int32.v (Some?.v (Seq.index (array_value_of var_r) (SizeT.v var_n)))) =
+optimal_revenue (to_nat_seq (array_value_of var_prices)) (SizeT.v var_n)))
+{
+  let mut var_prices = var_prices;
+  let mut var_n = var_n;
+  let mut var_r = var_r;
+  (array_write (!var_r) 0sz (Int32.int_to_t 0));
+  dp_correct_init
+(to_nat_seq (array_value_of (!var_prices)))
+(to_nat_seq (array_value_of (!var_r)));
+  let mut var_j : SizeT.t;
+  var_j := 1sz;
+  while (((!var_j) `SizeT.lte` (!var_n)))
+    invariant (live var_j)
+    invariant ((Pulse.Lib.C.Array.live_array (!var_r)) **
+        (Pulse.Lib.C.Array.live_array (!var_prices)))
+    invariant (with_pure
+        (((reveal (length_of (!var_r))) = ((SizeT.v (!var_n)) + 1)) &&
+          ((reveal (length_of (!var_prices))) = (SizeT.v (!var_n)))))
+    invariant (with_pure
+        ((1 <= (SizeT.v (!var_j))) && ((SizeT.v (!var_j)) <= ((SizeT.v (!var_n)) + 1))))
+    invariant (with_pure ((SizeT.v (!var_n)) <= 1000))
+    invariant (with_pure
+        (forall
+          (var_ii: SizeT.t).
+          (((!var_n) `SizeT.lte` var_ii) ||
+            ((0 <= (id #int (Int32.v ((array_read (!var_prices) var_ii))))) &&
+              ((id #int (Int32.v ((array_read (!var_prices) var_ii)))) <= 1000000)))))
+    invariant (with_pure (Int32.v (array_read (!var_r) 0sz) = 0))
+    invariant (with_pure
+        (forall
+          (var_k: SizeT.t).
+          (((!var_j) `SizeT.lte` var_k) ||
+            (0 <= (id #int (Int32.v ((array_read (!var_r) var_k))))))))
+    invariant (with_pure
+        (forall
+          (var_k: SizeT.t).
+          (((!var_j) `SizeT.lte` var_k) ||
+            (Int32.v (array_read (!var_r) var_k) <= 1000000 * SizeT.v var_k))))
+    invariant (with_pure (
+dp_correct
+(to_nat_seq (array_value_of (!var_prices)))
+(to_nat_seq (array_value_of (!var_r)))
+(SizeT.v (!var_j) - 1)))
+  {
+    let mut var_q : Int32.t;
+    var_q := (Int32.int_to_t 0);
+    let mut var_i : SizeT.t;
+    var_i := 1sz;
+    while (((!var_i) `SizeT.lte` (!var_j)))
+      invariant (((live var_i) ** (live var_q)) ** (live var_j))
+      invariant ((Pulse.Lib.C.Array.live_array (!var_r)) **
+          (Pulse.Lib.C.Array.live_array (!var_prices)))
+      invariant (with_pure
+          (((reveal (length_of (!var_r))) = ((SizeT.v (!var_n)) + 1)) &&
+            ((reveal (length_of (!var_prices))) = (SizeT.v (!var_n)))))
+      invariant (with_pure ((1 <= (SizeT.v (!var_j))) && ((!var_j) `SizeT.lte` (!var_n))))
+      invariant (with_pure
+          ((1 <= (SizeT.v (!var_i))) && ((SizeT.v (!var_i)) <= ((SizeT.v (!var_j)) + 1))))
+      invariant (with_pure ((SizeT.v (!var_n)) <= 1000))
+      invariant (with_pure
+          (forall
+            (var_ii: SizeT.t).
+            (((!var_n) `SizeT.lte` var_ii) ||
+              ((0 <= (id #int (Int32.v ((array_read (!var_prices) var_ii))))) &&
+                ((id #int (Int32.v ((array_read (!var_prices) var_ii)))) <= 1000000)))))
+      invariant (with_pure (Int32.v (array_read (!var_r) 0sz) = 0))
+      invariant (with_pure
+          (forall
+            (var_k: SizeT.t).
+            (((!var_j) `SizeT.lte` var_k) ||
+              (0 <= (id #int (Int32.v ((array_read (!var_r) var_k))))))))
+      invariant (with_pure
+          (forall
+            (var_k: SizeT.t).
+            (((!var_j) `SizeT.lte` var_k) ||
+              (Int32.v (array_read (!var_r) var_k) <= 1000000 * SizeT.v var_k))))
+      invariant (with_pure (0 <= (id #int (Int32.v (!var_q)))))
+      invariant (with_pure (Int32.v (!var_q) <= 1000000 * SizeT.v (!var_j)))
+      invariant (with_pure (
+dp_correct
+(to_nat_seq (array_value_of (!var_prices)))
+(to_nat_seq (array_value_of (!var_r)))
+(SizeT.v (!var_j) - 1)))
+      invariant (with_pure (
+id #int (Int32.v (!var_q)) ==
+accum_max
+(to_nat_seq (array_value_of (!var_prices)))
+(to_nat_seq (array_value_of (!var_r)))
+(SizeT.v (!var_j))
+(SizeT.v (!var_i) - 1)))
+    {
+      let mut var_p_val : Int32.t;
+      var_p_val := ((array_read (!var_prices) ((!var_i) `SizeT.sub` 1sz)));
+      let mut var_r_val : Int32.t;
+      var_r_val := ((array_read (!var_r) ((!var_j) `SizeT.sub` (!var_i))));
+      assert (with_pure (0 <= (id #int (Int32.v (!var_p_val)))));
+      assert (with_pure ((id #int (Int32.v (!var_p_val))) <= 1000000));
+      assert (with_pure (0 <= (id #int (Int32.v (!var_r_val)))));
+      assert (with_pure ((id #int (Int32.v (!var_r_val))) <= 999000000));
+      let mut var_candidate : Int32.t;
+      var_candidate := ((!var_p_val) `Int32.add` (!var_r_val));
+      if (((!var_q) `Int32.lt` (!var_candidate))) {
+        var_q := (!var_candidate);
+      } else {};
+      var_i := ((!var_i) `SizeT.add` 1sz);
+    };
+    accum_max_dp_correct
+(to_nat_seq (array_value_of (!var_prices)))
+(to_nat_seq (array_value_of (!var_r)))
+(SizeT.v (!var_j));
+    (array_write (!var_r) (!var_j) (!var_q));
+    var_j := ((!var_j) `SizeT.add` 1sz);
+  };
+}
